---
title: "Lista 1"
author: 
  - Álvaro Jerônimo da Silva Kothe
  - Larissa Porto Eleutério
date: "16/09/2021"
output: html_document
---


## Exercício 1

Prove a expressão
\[
cov(y, w) = cov_u(E(y|u), E(w|u)) + E_u(cov(y, w)|u)
\]

**Resposta:**

Como

$$
cov(y, w) = E[yw] - E(y)E(w),
$$
sabendo que $E(g) = E_y[E(g|y)]$

\[cov(y, w) = E_u[E(yw|u)] - E_u[E(y|u)] E_u[E(w|u)],\]

tomando que $E(yw|u) = cov(y, w|u) + E(y|u)E(w|u),$ temos que



\[\begin{split}
cov(y, w) &= E_u[cov(y, w|u) + E(y|u)E(w|u)] - E_u[E(y|u)] E_u[E(w|u)] \\
          &= E_u[cov(y, w|u)] + E_u[E(y|u)E(w|u)] - E_u[E(y|u)] E_u[E(w|u)],
\end{split}
\]

como $E_u[E(y|u)E(w|u)] - E_u[E(y|u)] E_u[E(w|u)] = cov_u(E(y|u), E(w|u))$

$\therefore cov(y, w) = E_u[cov(y, w|u)] + cov_u(E(y|u), E(w|u)).$

## Exercício 1 (seção 2.1)


## Exercício 2 (seção 2.1)


## Exercício 4 (seção 2.1)




